examples/formal-languages/regular/regexpLib.sml
@@ -2,14 +2,22 @@ structure regexpLib :> regexpLib =
 struct
 
 open HolKernel boolLib bossLib;
-open pairLib optionLib pred_setLib listLib stringLib;
+open pairLib optionLib pred_setLib listLib stringLib wordsLib;
 open listTheory stringTheory arithmeticTheory pred_setTheory 
      sortingTheory mergesortTheory comparisonTheory balanced_mapTheory 
-     charsetTheory regexpTheory vec_mapTheory regexp_compilerTheory; 
-open Regexp_Type regexpSyntax;
+     charsetTheory regexpTheory vec_mapTheory regexp_compilerTheory;
 
-fun stdOut_print s = let open TextIO in output(stdOut,s); flushOut stdOut end;
-fun stdErr_print s = let open TextIO in output(stdErr,s); flushOut stdErr end;
+open Regexp_Type regexpSyntax regexpMisc;
+
+fun sml_matcher r = 
+ let val {matchfn,start,table,final} = Regexp_Match.vector_matcher r
+     val _ = stdErr_print (Int.toString(Vector.length final)^" states.\n")
+ in {certificate = NONE:thm option,
+     matchfn = matchfn,
+     table = table,
+     start = start,
+     final = final}
+ end;
 
 (*---------------------------------------------------------------------------*)
 (* Proof-based compilation of regexps into DFAs, and associated regexp       *)
@@ -42,25 +50,21 @@ val vector_defs =
 val regexp_compute_thms = 
   vector_defs 
   @
-  [ALPHABET_def, alphabet_size_def, And_def,
-   zip_def, genlist_def, toListAux_def, toList_def,
-   vector_slice_cmp_def, vector_cmp_def,
-   len_cmp_def, bool_cmp_def,
-   all_unset_def, all_set_def, charset_empty_def, charset_full_def, 
-   charset_mem_def, charset_sing_def, 
-   charset_union_def, charset_insert_def, merge_charsets_def, charset_cmp_def,
-   numeral_cmp_thm, comparisonTheory.list_cmp_def,
-   
+  [ALPHABET_def, alphabet_size_def, And_def, zip_def,
+   charset_empty_def, charset_full_def, 
+   charset_mem_def, charset_union_def, charset_sing_def, merge_charsets_def, 
+
+   charset_cmp_def, numeral_cmp_thm, len_cmp_def, 
    regexp_compare_def,regexp_compareW_def,regexp_compare_eq,regexp_leq_def, 
 
    build_char_set_def, Sigma_def, Empty_def, Epsilon_def, catstring_def,
    assoc_cat_def, build_cat_def, build_neg_def, build_star_def, 
    flatten_or_def, remove_dups_def, build_or_def, 
-   nullable_def, nullableW_def, smart_deriv_def, normalize_def, 
+   nullable_def, nullableW_def, smart_deriv_thm, (* smart_deriv_def *) normalize_def, 
    transitions_def, build_table_def, extend_states_def,
    insert_regexp_def, mem_regexp_def, relationTheory.inv_image_def, 
 
-   dom_Brz_alt_eqns, SIMP_RULE bool_ss [dom_Brz_alt_equal] exec_Brz_def, 
+   dom_Brz_alt_eqns,SIMP_RULE bool_ss [dom_Brz_alt_equal] exec_Brz_def, 
    Brzozo_def, Brzozowski_exec_Brz, MAXNUM_32_def, 
    get_accepts_def, numLib.SUC_RULE (vec_mapTheory.alist_to_vec_def), 
    accepts_to_vector_def, table_to_vectors_def, 
@@ -78,10 +82,8 @@ val regexp_compute_thms =
    balanced_mapTheory.size_def,
    balanced_mapTheory.delta_def,
    balanced_mapTheory.foldrWithKey_def,
-
    (* adding stuff revealed by computeLib.unmapped *)
-   combinTheory.o_DEF, combinTheory.I_THM,   combinTheory.K_DEF, combinTheory.FAIL_DEF,
-   basicSizeTheory.bool_size_def,
+   combinTheory.o_DEF, combinTheory.I_THM, combinTheory.C_DEF, combinTheory.FAIL_DEF,
    rich_listTheory.SPLITP_AUX_def, rich_listTheory.SPLITP_compute,rich_listTheory.SEG_compute
  ];
 
@@ -95,12 +97,11 @@ fun regexp_compset() =
      val _ = optionLib.OPTION_rws compset
      val _ = pairLib.add_pair_compset compset
      val _ = pred_setLib.add_pred_set_compset compset
-(*     val _ = wordsLib.add_words_compset true compset *)
+     val _ = wordsLib.add_words_compset true compset
      val _ = stringLib.add_string_compset compset
      val _ = add_datatype_info compset (valOf(TypeBase.fetch ``:cpn``))
      val _ = add_datatype_info compset (valOf(TypeBase.fetch ``:regexp``))
      val _ = add_datatype_info compset (valOf(TypeBase.fetch ``:('a,'b)balanced_map``))
-     val _ = add_datatype_info compset (valOf(TypeBase.fetch ``:'a vector``))
      val _ = add_thms regexp_compute_thms compset
  in
    compset
@@ -112,65 +113,18 @@ fun regexp_compset() =
 
 val compset = regexp_compset();
 
-val unmapped_consts = computeLib.unmapped compset;
+val check_these_consts = computeLib.unmapped compset;
 
 val regexpEval = computeLib.CBV_CONV compset;
-
 
 (*
 max_print_depth := 25;
 
+fun compile q = 
+  regexpEval ``compile_regexp ^(mk_regexp(Regexp_Type.fromQuote q))``;
+
 val regexp_tm = mk_regexp(Regexp_Type.fromQuote `a`);
-
-regexpEval ``compile_regexp ^regexp_tm``;
-
-regexpEval ``exec_Brz empty [^regexp_tm] (1,singleton ^regexp_tm 0,[]) MAXNUM_32``;
-regexpEval ``transitions ^regexp_tm``;
-regexpEval ``insert_regexp ^regexp_tm empty``;
-regexpEval ``remove_dups (MAP SND (transitions ^regexp_tm))``;
-regexpEval ``build_table (transitions ^regexp_tm) ^regexp_tm (1,singleton ^regexp_tm 0,[])``;
-regexpEval ``extend_states 1n (singleton ^regexp_tm 0) [] (transitions ^regexp_tm)``;
-
-val (_,[next_state,state_map,trans,_]) = strip_comb ``extend_states 1n (singleton ^regexp_tm 0) [] (transitions ^regexp_tm)``;
-val arcs_tm = rhs(concl (regexpEval ``transitions ^regexp_tm``));
-val arcs = fst(listSyntax.dest_list arcs_tm);
-
-fun opr [] next_state state_map trans = ([],next_state,state_map,trans)
-  | opr (cr::t) next_state state_map trans = 
-     let val _ = print "."
-         val (c,r') = pairSyntax.dest_pair cr
-         val opt = rhs(concl (regexpEval ``lookup regexp_compare ^(r') ^state_map``))
-     in 
-       if optionSyntax.is_some opt
-        then let val n = optionSyntax.dest_some opt
-                 val trans = rhs(concl (regexpEval ``((^c,^n)::^trans)``))
-             in opr t next_state state_map trans
-             end
-        else let val next_state = rhs (concl (regexpEval ``^next_state + 1``))
-                 val state_map = rhs (concl (regexpEval ``insert regexp_compare ^(r') 1n ^state_map``))
-                 val trans = rhs(concl (regexpEval ``((^c,1n)::^trans)``))
-             in opr t next_state state_map trans
-             end
-     end;
-
-val res = opr arcs next_state state_map trans;
-
-extend_states_def
- |- extend_states next_state state_map trans [] = (next_state,state_map,trans)) ∧
-    extend_states next_state state_map trans ((c,r')::t) =
-     case lookup regexp_compare r' state_map
-      of NONE => extend_states 
-                  (next_state + 1)
-                  (insert regexp_compare r' next_state state_map)
-                  ((c,next_state)::trans)
-                  t
-     | SOME n => extend_states next_state state_map ((c,n)::trans) t:
-   thm
-
-
 *)
-
-(* Apply optimization for dom_Brz *)
 
 val Brzozowski_partial_eval_alt = 
    SIMP_RULE bool_ss [dom_Brz_alt_equal] Brzozowski_partial_eval;
@@ -209,14 +163,14 @@ fun hol_matcher r =
      val eq_tm = snd(strip_forall (concl dfa_thm))
      val (_,[final,table,start,_]) = strip_comb(boolSyntax.lhs eq_tm)
      val ifinal = List.map (equal boolSyntax.T) 
-                  (fst(dest_list (dest_vector final)))
+                  (fst(listSyntax.dest_list (dest_vector final)))
      val istart = numSyntax.int_of_term start
+     val rows1 = dest_vector table
      fun dest_row row = 
-        let val opts = fst (dest_list row)
+        let val opts = fst (listSyntax.dest_list row)
         in List.map (numSyntax.int_of_term o optionSyntax.dest_some) opts
         end
-     val rows1 = dest_vector table
-     val rows2 = fst(dest_list(snd(dest_map rows1)))
+     val rows2 = fst(listSyntax.dest_list(snd(listSyntax.dest_map rows1)))
      val itable = List.map dest_row rows2
      val len = length ifinal
      val _ = stdErr_print (Int.toString len^" states.\n")
@@ -228,28 +182,18 @@ fun hol_matcher r =
       final = Vector.fromList ifinal}
  end;
 
-fun sml_matcher r = 
- let val {matchfn,start,table,final} = Regexp_Match.vector_matcher r
-     val _ = stdErr_print (Int.toString(Vector.length final)^" states.\n")
- in {certificate = NONE:thm option,
-     matchfn = matchfn,
-     table = table,
-     start = start,
-     final = final}
- end;
 
 datatype evaluator = HOL | SML ;
 
 fun matcher HOL = hol_matcher 
   | matcher SML = sml_matcher;
 
-
-fun dfa_by_proof (name,q) = 
+fun dfa_by_proof (name,r) = 
  let val name = if Lexis.ok_identifier name then name
                else (HOL_MESG (Lib.quote name^
                        " is not a suitable identifier, using \"foo\" instead");
                      "foo")
-     val {certificate, start,table,final,matchfn} = hol_matcher (Regexp_Type.fromQuote q)
+     val {certificate, start,table,final,matchfn} = hol_matcher r
      val SOME thm = certificate
      val eqn = snd(dest_forall(concl thm))
      val (exec_dfa,[finals,table,start,s]) = strip_comb(lhs eqn)
